Proving Measurement. Loop 1 settled down.

AbstractPlatform/Measure.bpl
@@ -13,6 +13,18 @@ function valid_regindex_le(ri : regindex_t, rmax : regindex_t) : bool
 //--------------------------------------------------------------------------//
 // Helper fns in order to state measurement invariants.                     //
 //--------------------------------------------------------------------------//
+// valid PE structure: be same
+// notice case that eid == root1/2
+function {:inline} encl_owner_map_match(valid1 : tap_enclave_metadata_valid_t,
+                                        valid2 : tap_enclave_metadata_valid_t,
+                                        map1 : tap_enclave_metadata_owner_map_t, 
+                                        map2 : tap_enclave_metadata_owner_map_t, 
+                                        eid : tap_enclave_id_t,
+                                        root1 : tap_enclave_id_t, 
+                                        root2 : tap_enclave_id_t) : bool
+{ (valid1[eid] && map1[eid] == root1) <==> (valid2[eid] && map2[eid] == root2) }
+
+
 function {:inline} excl_match(ev1 : excl_vaddr_t, ev2 : excl_vaddr_t, v : vaddr_t) : bool
 { ev1[v] == ev2[v] }
 
@@ -74,11 +86,24 @@ function {:inline} update_digest_virt_addr(
   //       else update_digest(1, s))
   //  else update_digest(k0_measurement_t, s)
 
+// int(2)
 const kbias_cpu_measurement_index : int;
 axiom kbias_cpu_measurement_index == 2;
 
+const kbias_privil_measurement_index : int;
+axiom kbias_privil_measurement_index == 1;
+
+// int(2 + 512)
+const kmax_cpu_regs_bound_index : int;
+axiom kmax_cpu_regs_bound_index == kbias_cpu_measurement_index + kN_regindex_t_as_int;
+
+// int(2 + 512 + 1)
+const kmax_cpu_privil_bound_index : int;
+axiom kmax_cpu_privil_bound_index == kbias_privil_measurement_index + kmax_cpu_regs_bound_index;
+
+// int(2 + 512 + 1 + 512)
 const kmax_cpu_measurement_index : int;
-axiom kmax_cpu_measurement_index == kbias_cpu_measurement_index + kN_regindex_t_as_int;
+axiom kmax_cpu_measurement_index == kmax_cpu_privil_bound_index + kN_enclave_id_t;
 
 /* append metadata: privileged */ 
 procedure {:inline 1} measure_cpu_state_at_index(
@@ -87,6 +112,9 @@ procedure {:inline 1} measure_cpu_state_at_index(
    /* pc         */ pc         : vaddr_t          , 
    /* entrypoint */ entrypoint : vaddr_t          ,
    /* index      */ index      : int              ,
+   /* privileged */ privileged : bool             ,
+   /* owner_map  */ ownermap   : tap_enclave_metadata_owner_map_t,
+   /* encl valid */ valid      : tap_enclave_metadata_valid_t,
    /* meas in    */ s          : measurement_t
 )
   returns (t : measurement_t)
@@ -95,6 +123,7 @@ procedure {:inline 1} measure_cpu_state_at_index(
 {
   var ri : regindex_t;
   var vi : int;
+  var iter_eid : tap_enclave_id_t;
 
   if (index == 0) {
     t := update_digest(vaddr2int(pc), s);
@@ -102,13 +131,23 @@ procedure {:inline 1} measure_cpu_state_at_index(
   else if (index == 1) {
     t := update_digest(vaddr2int(entrypoint), s);
   } 
-  // else if (index == 2) {
-  //   t := update_digest(privileged2int(tap_enclave_metadata_privileged[eid]), s);
-  // } 
-  else if (index >= kbias_cpu_measurement_index && index < kmax_cpu_measurement_index) {
+  else if (index >= kbias_cpu_measurement_index && index < kmax_cpu_regs_bound_index) {
     ri := index - kbias_cpu_measurement_index;
     assert valid_regindex(ri);
     t := update_digest(word2int(regs[ri]), s);
+  } 
+  else if (index >= kmax_cpu_regs_bound_index && index < kmax_cpu_privil_bound_index) {
+    t := update_digest(bool2int(privileged), s); 
+  }
+  else if (index >= kmax_cpu_privil_bound_index && index < kmax_cpu_measurement_index) {
+    iter_eid := index - kmax_cpu_privil_bound_index;
+    assert valid_enclave_id_index(eid);
+    if (valid[iter_eid] && ownermap[iter_eid] == eid) {
+      // iter_eid cannot be tap_null_enc_id, avoid default value
+      t := update_digest(iter_eid, s);
+    } else {
+      t := update_digest(k0_int_t, s);
+    }
   }
 }
 
@@ -125,75 +164,134 @@ procedure measure_state_self_composed(
      /* mem        */ m1          , m2          : mem_t            , 
      /* regs       */ regs1       , regs2       : regs_t           , 
      /* pc         */ pc1         , pc2         : vaddr_t          , 
-     /* entrypoint */ entrypoint1 , entrypoint2 : vaddr_t
+     /* entrypoint */ entrypoint1 , entrypoint2 : vaddr_t          ,
+     /* privileged */ privileged1 , privileged2 : bool             ,
+     /* ownermap   */ ownermap1   , ownermap2   : tap_enclave_metadata_owner_map_t,
+     /* encl valid */ valid1      , valid2      : tap_enclave_metadata_valid_t
 )
   returns (t1 : measurement_t, t2 : measurement_t)
-  ensures ((forall v : vaddr_t :: 
+  // some additional requirement on ownermap structure.
+  // These 2 judge conditions could be merged.
+  requires (valid_enclave_id_index(e1) && valid_enclave_id_index(e2));
+  requires (valid_enclave_id(e1) && valid_enclave_id(e2));
+  requires (ownermap1[tap_null_enc_id] == tap_null_enc_id);
+  requires (ownermap2[tap_null_enc_id] == tap_null_enc_id);
+
+  ensures ((forall v : vaddr_t :: (GE_va(v, k0_vaddr_t) && LE_va(v, kmax_vaddr_t)) ==>
               (excl_match(ev1, ev2, v)                                                 &&
                addr_valid_match(ev1, ev2, av1, av2, v)                                 &&
                private_data_match(ev1, ev2, am1, am2, m1, m2, v)))                     &&
            (forall ri : regindex_t :: valid_regindex(ri) ==> (regs1[ri] == regs2[ri])) &&
-           (pc1 == pc2 && entrypoint1 == entrypoint2))
+           (pc1 == pc2 && entrypoint1 == entrypoint2 && privileged1 == privileged2)    &&
+           (forall e : tap_enclave_id_t :: valid_enclave_id_index(e) ==>
+              encl_owner_map_match(valid1, valid2, ownermap1, ownermap2, e, e1, e2)))
           <==> (t1 == t2);
-  ensures ((exists v : vaddr_t :: 
+  ensures ((exists v : vaddr_t :: (GE_va(v, k0_vaddr_t) && LE_va(v, kmax_vaddr_t)) &&
               (!excl_match(ev1, ev2, v)                                               ||
                !addr_valid_match(ev1, ev2, av1, av2, v)                               ||
                !private_data_match(ev1, ev2, am1, am2, m1, m2, v)))                   ||
            (exists ri : regindex_t :: valid_regindex(ri) && (regs1[ri] != regs2[ri])) ||
-           (pc1 != pc2 || entrypoint1 != entrypoint2))
+           (pc1 != pc2 || entrypoint1 != entrypoint2 || privileged1 != privileged2)   || 
+           (exists e : tap_enclave_id_t :: valid_enclave_id_index(e) &&
+              !encl_owner_map_match(valid1, valid2, ownermap1, ownermap2, e, e1, e2)))
           <==> (t1 != t2);
 {
   var index : int;
   var va    : vaddr_t;
-
+  // Loop 1. update digest/measurement by cpu state and metadata.
+  // A stronger assume: e1 == e2 ==> digest1 == digest2
   t1 := 0; t2 := 0; index := 0;
   while (index < kmax_cpu_measurement_index)
     invariant (index >= 0 && index <= kmax_cpu_measurement_index);
-    invariant ((pc1 == pc2 && entrypoint1 == entrypoint2 && e1 == e2)                    &&
+    invariant ((pc1 == pc2 && entrypoint1 == entrypoint2 && e1 == e2 && privileged1 == privileged2) &&
                (forall ri : regindex_t :: valid_regindex(ri) ==> regs1[ri] == regs2[ri]) &&
-               (forall v : vaddr_t :: av1[v] == av2[v] && am1[v] == am2[v]))
+               (forall v : vaddr_t :: av1[v] == av2[v] && am1[v] == am2[v]) &&
+               (forall e : tap_enclave_id_t :: valid_enclave_id_index(e) ==> 
+                  encl_owner_map_match(valid1, valid2, ownermap1, ownermap2, e, e1, e2)))
               ==> (t1 == t2);
+    // Step by step.
+    // 1 step over: pc
     invariant (index >= 1) ==> ((pc1 != pc2) ==> (t1 != t2));
     invariant (index <= 1) ==> ((pc1 == pc2) ==> (t1 == t2));
-    invariant (index >= 2) ==> ((entrypoint1 != entrypoint2) ==> (t1 != t2));
-    invariant (index <= 2) ==> (((pc1 == pc2) && (entrypoint1 == entrypoint2)) ==> (t1 == t2));
-    invariant (index >= 2) ==> 
-                ((exists ri : regindex_t :: 
-                    (valid_regindex(ri) && ri < (index-2) && (regs1[ri] != regs2[ri]))) 
-                        ==> (t1 != t2));
-    invariant (index >= 3) ==> 
-          (((pc1 == pc2) && (entrypoint1 == entrypoint2) &&
-            (forall ri : regindex_t :: 
-                (valid_regindex(ri) && ri < (index-2)) ==> (regs1[ri] == regs2[ri])))
-          ==> (t1 == t2));
+    // 2 steps over: entry
+    invariant (index >= kbias_cpu_measurement_index) ==> ((entrypoint1 != entrypoint2) ==> (t1 != t2));
+    invariant (index <= kbias_cpu_measurement_index) ==> (((pc1 == pc2) && (entrypoint1 == entrypoint2)) ==> (t1 == t2));
+    // 2+n (n<=512) steps over: regs
+    invariant (index > kbias_cpu_measurement_index && index <= kmax_cpu_regs_bound_index) ==> 
+                ((pc1 == pc2) && (entrypoint1 == entrypoint2) && 
+                 (forall ri : regindex_t :: 
+                      (valid_regindex(ri) && ri < index - kbias_cpu_measurement_index) ==> regs1[ri] == regs2[ri]) 
+                          ==> (t1 == t2));
+    invariant (index > kbias_cpu_measurement_index) ==> 
+              ((exists ri : regindex_t :: 
+                  (valid_regindex(ri) && ri < (index - kbias_cpu_measurement_index) && (regs1[ri] != regs2[ri]))) 
+                      ==> (t1 != t2));
+    invariant (index >= kmax_cpu_regs_bound_index) ==> 
+                ((exists ri : regindex_t :: valid_regindex(ri) && 
+                  regs1[ri] != regs2[ri]) ==> (t1 != t2));
+    // 2+512+1 steps over: privilege tag
+    invariant (index > kmax_cpu_regs_bound_index && index <= kmax_cpu_privil_bound_index) ==> 
+                ((pc1 == pc2) && (entrypoint1 == entrypoint2) && (privileged1 == privileged2) && 
+                 (forall ri : regindex_t :: 
+                       valid_regindex(ri) ==> regs1[ri] == regs2[ri]) 
+                          ==> (t1 == t2));    
+    invariant (index > kmax_cpu_regs_bound_index) ==> 
+              ((privileged1 != privileged2) ==> (t1 != t2));
+    // 2+512+1+n (n<=512) steps over: ownermap
+    invariant (index > kmax_cpu_privil_bound_index && index <= kmax_cpu_measurement_index) ==> 
+                ((pc1 == pc2) && (entrypoint1 == entrypoint2) && (privileged1 == privileged2) && 
+                 (forall ri : regindex_t :: 
+                       valid_regindex(ri) ==> regs1[ri] == regs2[ri]) &&
+                 (forall e : tap_enclave_id_t :: 
+                      (valid_enclave_id_index(e) && e < index - kmax_cpu_privil_bound_index) ==> 
+                          encl_owner_map_match(valid1, valid2, ownermap1, ownermap2, e, e1, e2)) 
+                              ==> (t1 == t2));
+    invariant (index > kmax_cpu_privil_bound_index) ==> 
+              ((exists e : tap_enclave_id_t :: 
+                      ( valid_enclave_id_index(e) && 
+                        e < index - kmax_cpu_privil_bound_index && 
+                       !encl_owner_map_match(valid1, valid2, ownermap1, ownermap2, e, e1, e2))) 
+                          ==> (t1 != t2));
   {
-    call t1 := measure_cpu_state_at_index(e1, regs1, pc1, entrypoint1, index, t1);
-    call t2 := measure_cpu_state_at_index(e2, regs2, pc2, entrypoint2, index, t2);
+    call t1 := measure_cpu_state_at_index(e1, regs1, pc1, entrypoint1, index, privileged1, ownermap1, valid1, t1);
+    call t2 := measure_cpu_state_at_index(e2, regs2, pc2, entrypoint2, index, privileged2, ownermap2, valid2, t2);
     index := index + 1;
   }
   assert ((forall ri : regindex_t :: valid_regindex(ri) ==> (regs1[ri] == regs2[ri])) &&
-          pc1 == pc2 && entrypoint1 == entrypoint2)
+          pc1 == pc2 && entrypoint1 == entrypoint2 && privileged1 == privileged2 && 
+          (forall e : tap_enclave_id_t :: valid_enclave_id_index(e) ==> 
+              encl_owner_map_match(valid1, valid2, ownermap1, ownermap2, e, e1, e2)))
          <==> (t1 == t2);
   assert ((exists ri : regindex_t :: valid_regindex(ri) && (regs1[ri] != regs2[ri])) ||
-          pc1 != pc2 || entrypoint1 != entrypoint2)
+          pc1 != pc2 || entrypoint1 != entrypoint2 || privileged1 != privileged2 || 
+          (exists e : tap_enclave_id_t :: valid_enclave_id_index(e) && 
+              !encl_owner_map_match(valid1, valid2, ownermap1, ownermap2, e, e1, e2)))
          <==> (t1 != t2);
+  
+  // Loop 2. update digest/measurement by v
 
   va := k0_vaddr_t;
   while (LT_va(va, kmax_vaddr_t)) 
+    // buggy claims
     invariant ((forall ri : regindex_t :: valid_regindex(ri) ==> (regs1[ri] == regs2[ri])) &&
-               pc1 == pc2 && entrypoint1 == entrypoint2 &&
-               (forall v : vaddr_t :: LT_va(v, va) ==> 
-                  (excl_match(ev1, ev2, v)                                                 &&
-                   addr_valid_match(ev1, ev2, av1, av2, v)                                 &&
-                   private_data_match(ev1, ev2, am1, am2, m1, m2, v))))
+               pc1 == pc2 && entrypoint1 == entrypoint2 && privileged1 == privileged2      &&
+               (forall v : vaddr_t :: 
+                  (LT_va(v, va) && GE_va(v, k0_vaddr_t) && LE_va(v, kmax_vaddr_t)) ==> 
+                      (excl_match(ev1, ev2, v)                                             &&
+                      addr_valid_match(ev1, ev2, av1, av2, v)                              &&
+                      private_data_match(ev1, ev2, am1, am2, m1, m2, v)))                  &&
+               (forall e : tap_enclave_id_t :: valid_enclave_id_index(e) ==>
+                  encl_owner_map_match(valid1, valid2, ownermap1, ownermap2, e, e1, e2)))
                ==> (t1 == t2);
     invariant ((exists ri : regindex_t :: valid_regindex(ri) && (regs1[ri] != regs2[ri])) ||
-               pc1 != pc2 || entrypoint1 != entrypoint2 || 
+               pc1 != pc2 || entrypoint1 != entrypoint2 || privileged1 != privileged2 ||
                (exists v : vaddr_t :: 
-                   LT_va(v, va) && 
+                   (LT_va(v, va) && GE_va(v, k0_vaddr_t) && LE_va(v, kmax_vaddr_t)) && 
                       (!excl_match(ev1, ev2, v)                                               ||
                        !addr_valid_match(ev1, ev2, av1, av2, v)                               ||
-                       !private_data_match(ev1, ev2, am1, am2, m1, m2, v))))
+                       !private_data_match(ev1, ev2, am1, am2, m1, m2, v)))                   ||
+               (exists e : tap_enclave_id_t :: valid_enclave_id_index(e) &&
+                  !encl_owner_map_match(valid1, valid2, ownermap1, ownermap2, e, e1, e2)))
                ==> (t1 != t2);
   {
     t1 := update_digest_virt_addr(av1, am1, ev1, m1, va, t1);
@@ -207,6 +305,7 @@ procedure measure_state_self_composed(
 //--------------------------------------------------------------------------//
 // Measurement API                                                          //
 //--------------------------------------------------------------------------//
+// Deprecated in measurement proof. Use measurement-self-composed instead.
 procedure {:inline 1} measure()
     returns (status : enclave_op_result_t, measurement : measurement_t)
 {
@@ -227,7 +326,13 @@ procedure {:inline 1} measure()
                                     tap_enclave_metadata_pc[cpu_enclave_id], 
                                     tap_enclave_metadata_pc[cpu_enclave_id], 
                                     tap_enclave_metadata_entrypoint[cpu_enclave_id],
-                                    tap_enclave_metadata_entrypoint[cpu_enclave_id]);
+                                    tap_enclave_metadata_entrypoint[cpu_enclave_id],
+                                    tap_enclave_metadata_privileged_1[cpu_enclave_id],
+                                    tap_enclave_metadata_privileged_2[cpu_enclave_id],
+                                    tap_enclave_metadata_owner_map_1,
+                                    tap_enclave_metadata_owner_map_2,
+                                    tap_enclave_metadata_valid_1,
+                                    tap_enclave_metadata_valid_2);
     assert measurement == temp;
     status := enclave_op_success;
 }
